interpreter/Interpreter/Wasm/Wp/Call.lean
@@ -202,6 +202,7 @@ theorem FuncSpec.of_wp_body
   | Trap msg => rw [hexec] at hQ; exact hQ.elim
   | Invalid msg => rw [hexec] at hQ; exact hQ.elim
   | OutOfFuel => rw [hexec] at hQ; exact hQ.elim
+  | ReturnCall fid st' vs => rw [hexec] at hQ; exact hQ.elim
 
 /-! ### Host calls.
 
